restore pre- and post-conditions in Lib.PQ.Buffer

lib/fst/Lib.PQ.Buffer.fst
@@ -2,13 +2,18 @@ module Lib.PQ.Buffer
 
 open FStar.HyperStack
 open FStar.HyperStack.ST
-module ST = FStar.HyperStack.ST
 open Lib.IntTypes
 open Lib.RawIntTypes
-open Lib.Sequence
+open LowStar.ModifiesPat
+open LowStar.Modifies
 
 module Buf = LowStar.Buffer
 module U32 = FStar.UInt32
+module ST = FStar.HyperStack.ST
+module HS = FStar.HyperStack
+
+module LSeq = Lib.Sequence
+module Seq = FStar.Seq
 
 unfold let v = size_v
 
@@ -19,42 +24,30 @@ val sub:
   #a:Type0 -> #len:size_nat -> #olen:size_nat ->
   b:lbuffer a len -> start:size_t ->
   n:size_t{v start + v n <= len /\ v n == olen} -> Stack (lbuffer a olen)
-  (requires (fun h0 -> True))
-  (ensures (fun h0 r h1 -> True))
+  (requires (fun h0 -> Buf.live h0 b))
+  (ensures (fun h0 r h1 -> h0 == h1 /\ r == Buf.gsub b (size_to_UInt32 start) (size_to_UInt32 n)))
 let sub #a #len #olen b start n =
-  admit();
   Buf.sub b (size_to_UInt32 start) (size_to_UInt32 n)
-
-inline_for_extraction
-val slice:
-  #a:Type0 -> #len:size_nat -> #olen:size_nat ->
-  b:lbuffer a len -> start:size_t ->
-  fin:size_t{v start <= v fin /\ v fin <= len /\ v fin - v start == olen} -> Stack (lbuffer a olen)
-  (requires (fun h0 -> True))
-  (ensures (fun h0 r h1 -> True))
-let slice #a #len #olen b start n =
-  admit();
-  Buf.sub b (size_to_UInt32 start) (size_to_UInt32 (n -. start))
 
 inline_for_extraction
 val index:
   #a:Type0 -> #len:size_nat ->
-  b:lbuffer a (len) -> i:size_t{v i < len} -> Stack a
-  (requires (fun h0 -> True))
-  (ensures (fun h0 r h1 -> True))
+  b:lbuffer a len -> i:size_t{v i < len} -> Stack a
+  (requires (fun h0 -> Buf.live h0 b))
+  (ensures (fun h0 r h1 -> h0 == h1 /\ r == Seq.index (Buf.as_seq h1 b) (v i)))
 let index #a #len b i =
-  admit();
   Buf.index b (size_to_UInt32 i)
 
 inline_for_extraction
 val upd:
-  #a:Type0 -> #len:size_nat ->
-  b:lbuffer a (len) -> i:size_t{v i < len} ->
+  #a:Type0 -> #len:size_nat{len > 0} ->
+  b:lbuffer a len -> i:size_t{v i < len} ->
   x:a -> Stack unit
-  (requires (fun h0 -> True))
-  (ensures (fun h0 r h1 -> True))
+  (requires (fun h0 -> Buf.live h0 b))
+  (ensures (fun h0 _ h1 ->
+    Buf.modifies_1 b h0 h1 /\ Buf.live h1 b /\
+    Buf.as_seq h1 b == Seq.upd (Buf.as_seq h0 b) (v i) x))
 let upd #a #len b i v =
-  admit();
   Buf.upd b (size_to_UInt32 i) v
 
 inline_for_extraction let op_Array_Assignment #a #len = upd #a #len
@@ -62,78 +55,122 @@ inline_for_extraction let op_Array_Access #a #len = index #a #len
 
 inline_for_extraction
 val create:
-  #a:Type0 -> #len:size_nat ->
+  #a:Type0 -> #len:size_nat{len > 0} ->
   clen:size_t{v clen == len} -> init:a -> StackInline (lbuffer a len)
   (requires (fun h0 -> True))
-  (ensures (fun h0 r h1 -> True))
+  (ensures (fun h0 r h1 ->
+    Buf.alloc_post_common (HS.get_tip h0) len r h0 h1 /\
+    Buf.as_seq h1 r == Seq.create len init))
 let create #a #len clen init =
-  admit();
   Buf.alloca init (size_to_UInt32 clen)
 
 inline_for_extraction
 val createL:
   #a:Type0 -> init:list a{List.Tot.length init <= max_size_t} ->
   StackInline (lbuffer a (List.Tot.length init))
-  (requires (fun h0 -> True))
-  (ensures (fun h0 r h1 -> True))
+  (requires (fun h0 -> Buf.alloc_of_list_pre #a init))
+  (ensures (fun h0 r h1 ->
+    let len = FStar.List.Tot.length init in
+    Buf.alloc_post_common (HS.get_tip h0) len r h0 h1 /\
+    Buf.as_seq h1 r == Seq.of_list init /\
+    Buf.alloc_of_list_post #a len r))
 let createL #a init =
-  admit();
   Buf.alloca_of_list init
 
 inline_for_extraction
 val createL_global:
   #a:Type0 -> init:list a{List.Tot.length init <= max_size_t} ->
   ST (lbuffer a (List.Tot.length init))
-  (requires fun h0 -> True)
-  (ensures  fun h0 r h1 -> True)
+  (requires fun h0 -> Buf.alloc_of_list_pre #a init)
+  (ensures  fun h0 r h1 ->
+    let len = FStar.List.Tot.length init in
+    Buf.alloc_post_common HyperStack.root len r h0 h1 /\
+    Buf.as_seq h1 r == Seq.of_list init)
 let createL_global #a init =
-  admit();
   Buf.gcmalloc_of_list HyperStack.root init
+
+// val lemma_seq_slice_index:
+//   #a:Type -> s1:Seq.seq a ->
+//   s2:Seq.seq a{Seq.length s1 = Seq.length s2} ->
+//   j:nat{j < Seq.length s1} -> Lemma
+//   (requires ((Seq.slice s1 0 j == Seq.slice s2 0 j) /\ (Seq.index s1 j == Seq.index s2 j)))
+//   (ensures  (Seq.slice s1 0 (j + 1) == Seq.slice s2 0 (j + 1)))
+// let lemma_seq_slice_index #a s1 s2 j =
+//   Seq.snoc_slice_index s1 0 j;
+//   Seq.snoc_slice_index s2 0 j
+
+// inline_for_extraction
+// val copy:
+//   #a:Type -> #len:size_nat ->
+//   o:lbuffer a len -> clen:size_t{v clen == len} ->
+//   i:lbuffer a len -> Stack unit
+//   (requires (fun h0 -> Buf.live h0 o /\ Buf.live h0 i /\ Buf.disjoint i o))
+//   (ensures (fun h0 _ h1 ->
+//     Buf.live h1 o /\ Buf.live h1 i /\ modifies (loc_buffer o) h0 h1 /\
+//     Buf.as_seq h1 o == Buf.as_seq h0 i))
+// let copy #a #len o clen i =
+//   let h0 = ST.get() in
+//   let inv (h1:mem) (j:nat{j <= len}) =
+//     Buf.live h1 o /\ Buf.live h1 i /\
+//     modifies (loc_buffer o) h0 h1 /\
+//     Seq.slice (Buf.as_seq h1 o) 0 j == Seq.slice (Buf.as_seq h0 i) 0 j in
+//   let f' (j:size_t{0 <= v j /\ v j < len}) : Stack unit
+//       (requires (fun h -> inv h (v j)))
+//       (ensures (fun h1 _ h2 -> inv h2 (v j + 1))) =
+//       let h1 = ST.get () in
+//       let src_i = i.(j) in
+//       o.(j) <- src_i;
+//       let h2 = ST.get () in
+//       lemma_seq_slice_index (Buf.as_seq h2 o) (Buf.as_seq h0 i) (v j);
+//       modifies_trans (loc_buffer o) h0 h1 (loc_buffer o) h2 in
+//   Lib.Loops.for (size 0) clen inv f'
 
 inline_for_extraction
 val copy:
   #a:Type -> #len:size_nat ->
   o:lbuffer a len -> clen:size_t{v clen == len} ->
   i:lbuffer a len -> Stack unit
-  (requires (fun h0 -> True))
-  (ensures (fun h0 _ h1 -> True))
+  (requires (fun h0 -> Buf.live h0 o /\ Buf.live h0 i /\ Buf.disjoint i o))
+  (ensures (fun h0 _ h1 ->
+    Buf.live h1 o /\ Buf.live h1 i /\ modifies (loc_buffer o) h0 h1 /\
+    Buf.as_seq h1 o == Buf.as_seq h0 i))
 let copy #a #len o clen i =
-  admit();
-  let h0 = ST.get() in
-  let inv (h1:mem) (j:nat) = True in
-  let f' (j:size_t{0 <= v j /\ v j <= len}) : Stack unit
-      (requires (fun h -> inv h (v j)))
-      (ensures (fun h1 _ h2 -> inv h2 (v j + 1))) =
-      let src_i = i.(j) in
-      o.(j) <- src_i in
-  Lib.Loops.for (size 0) clen inv f'
+  let h0 = ST.get () in
+  LowStar.BufferOps.blit i (size_to_UInt32 (size 0)) o (size_to_UInt32 (size 0)) (size_to_UInt32 clen);
+  let h1 = ST.get () in
+  assert (Seq.slice (Buf.as_seq h1 o) 0 len == Seq.slice (Buf.as_seq h0 i) 0 len)
+
+let loop_nospec_inv (#a:Type) (h0:mem) (h1:mem)
+		    (len:size_nat) (n:size_nat)
+		    (buf:lbuffer a len) (i:size_nat{i <= n}): Type =
+   Buf.live h0 buf /\ Buf.live h1 buf /\ modifies (loc_buffer buf) h0 h1
 
 inline_for_extraction
 val loop_nospec:
   #h0:mem -> #a:Type0 -> #len:size_nat ->
   n:size_t -> buf:lbuffer a len ->
-  impl:(i:size_t{v i < v n} ->
-	Stack unit (requires fun h0 -> True) (ensures  fun h0 r h1 -> True)) -> Stack unit
-  (requires (fun h -> True))
-  (ensures (fun _ _ h1 -> True))
+  impl:
+    (i:size_t{v i < v n} -> Stack unit
+      (requires fun h -> loop_nospec_inv #a h0 h len (v n) buf (v i))
+      (ensures  fun _ r h1 -> loop_nospec_inv #a h0 h1 len (v n) buf (v i + 1))) -> Stack unit
+  (requires (fun h -> h0 == h /\ Buf.live h0 buf))
+  (ensures (fun _ _ h1 -> Buf.live h1 buf /\ modifies (loc_buffer buf) h0 h1))
 let loop_nospec #h0 #a #len n buf impl =
-  admit();
-  let inv (h1:mem) (j:nat) = True in
-  let f' (j:size_t{0 <= v j /\ v j <= len}) : Stack unit
+  let inv (h1:mem) (j:nat{j <= v n}) =
+    loop_nospec_inv #a h0 h1 len (v n) buf j in
+  let f' (j:size_t{0 <= v j /\ v j < v n}): Stack unit
       (requires (fun h -> inv h (v j)))
-      (ensures (fun h1 _ h2 -> inv h2 (v j + 1))) =
+      (ensures (fun _ _ h2 -> inv h2 (v j + 1))) =
       impl j in
   Lib.Loops.for (size 0) n inv f'
-
-
 
 inline_for_extraction
 val uint_from_bytes_le:
   #t:m_inttype ->
   i:lbuffer uint8 (numbytes t) ->
   Stack (uint_t t)
-  (requires (fun h0 -> True))
-  (ensures (fun h0 o h1 -> True))
+  (requires (fun h0 -> Buf.live h0 i))
+  (ensures (fun h0 o h1 -> h0 == h1 /\ Buf.live h1 i))
 let uint_from_bytes_le #t i =
   admit();
   match t with
@@ -147,8 +184,8 @@ inline_for_extraction
 val uint_from_bytes_be:
   #t:m_inttype ->
   i:lbuffer uint8 (numbytes t) -> Stack (uint_t t)
-  (requires (fun h0 -> True))
-  (ensures (fun h0 o h1 -> True))
+  (requires (fun h0 -> Buf.live h0 i))
+  (ensures (fun h0 o h1 -> h0 == h1 /\ Buf.live h1 i))
 let uint_from_bytes_be #t i =
   admit();
   match t with
@@ -163,8 +200,8 @@ val uint_to_bytes_le:
   #t:m_inttype ->
   o:lbuffer uint8 (numbytes t) ->
   i:uint_t t -> Stack unit
-  (requires (fun h0 -> True))
-  (ensures (fun h0 _ h1 -> True))
+  (requires (fun h0 -> Buf.live h0 o))
+  (ensures (fun h0 _ h1 -> Buf.live h1 o /\ modifies (loc_buffer o) h0 h1))
 let uint_to_bytes_le #t o i =
   admit();
   match t with
@@ -179,8 +216,8 @@ val uint_to_bytes_be:
   #t:m_inttype ->
   o:lbuffer uint8 (numbytes t) ->
   i:uint_t t -> Stack unit
-  (requires (fun h0 -> True))
-  (ensures (fun h0 _ h1 -> True))
+  (requires (fun h0 -> Buf.live h0 o))
+  (ensures (fun h0 _ h1 -> Buf.live h1 o /\ modifies (loc_buffer o) h0 h1))
 let uint_to_bytes_be #t o i =
   admit();
   match t with
@@ -190,6 +227,6 @@ let uint_to_bytes_be #t o i =
   | U64 -> C.store64_be o (u64_to_UInt64 i)
   | U128 -> C.store128_be o (u128_to_UInt128 i)
 
-assume val print_compare_display: 
-  len:size_t -> lbuffer uint8 (size_v len) -> 
+assume val print_compare_display:
+  len:size_t -> lbuffer uint8 (size_v len) ->
   lbuffer uint8 (size_v len) -> Stack unit (requires (fun h -> True)) (ensures (fun h0 _ h1 -> True))
